src/NonlinearArithmetic/Internals/MulInternals.dfy
@@ -20,64 +20,64 @@ module MulInternals {
   import opened MulInternalsNonlinear
 
   /* performs multiplication for positive integers using recursive addition */
-  function {:opaque} mul_pos(x: int, y: int) : int
+  function {:opaque} mulPos(x: int, y: int) : int
     requires x >= 0
   {
     if x == 0 then 0
-    else y + mul_pos(x - 1, y)
+    else y + mulPos(x - 1, y)
   }
 
   /* performs multiplication for both positive and negative integers */ 
-  function mul_recursive(x: int, y: int) : int
+  function mulRecursive(x: int, y: int) : int
   {
-    if x >= 0 then mul_pos(x, y)
-    else -1 * mul_pos(-1 * x, y)
+    if x >= 0 then mulPos(x, y)
+    else -1 * mulPos(-1 * x, y)
   }
 
   /* performs induction on multiplication */ 
-  lemma lemma_mul_induction(f: int -> bool)
+  lemma lemmaMulInduction(f: int -> bool)
     requires f(0)
     requires forall i {:trigger f(i), f(i + 1)} :: i >= 0 && f(i) ==> f(i + 1)
     requires forall i {:trigger f(i), f(i - 1)} :: i <= 0 && f(i) ==> f(i - 1)
     ensures  forall i {:trigger f(i)} :: f(i)
   {
-    forall i ensures f(i) { lemma_induction_helper(1, f, i); }
+    forall i ensures f(i) { lemmaInductionHelper(1, f, i); }
   }
 
   /* proves that multiplication is always commutative */
-  lemma lemma_mul_commutes()
+  lemma lemmaMulCommutes()
     ensures  forall x:int, y:int {:trigger x * y} :: x * y == y * x
   {
     forall x:int, y:int
       ensures x * y == y * x
     {
-      lemma_mul_induction(i => x * i == i * x);
+      lemmaMulInduction(i => x * i == i * x);
     }
   }
 
   /* proves the distributive property of multiplication when multiplying an interger
   by (x +/- 1) */
   //rename for both directions ???
-  lemma lemma_mul_successor()
+  lemma lemmaMulSuccessor()
     ensures forall x:int, y:int {:trigger (x + 1) * y} :: (x + 1) * y == x * y + y
     ensures forall x:int, y:int {:trigger (x - 1) * y} :: (x - 1) * y == x * y - y
   {
-    lemma_mul_commutes();
+    lemmaMulCommutes();
     forall x:int, y:int
       ensures (x + 1) * y == x * y + y
       ensures (x - 1) * y == x * y - y
     {
-      lemma_mul_is_distributive_add(y, x, 1);
-      lemma_mul_is_distributive_add(y, x, -1);
+      lemmaMulIsDistributiveAdd(y, x, 1);
+      lemmaMulIsDistributiveAdd(y, x, -1);
     }
   }
 
   /* proves the distributive property of multiplication */
-  lemma lemma_mul_distributes()
+  lemma lemmaMulDistributes()
     ensures forall x:int, y:int, z:int {:trigger (x + y) * z} :: (x + y) * z == x * z + y * z
     ensures forall x:int, y:int, z:int {:trigger (x - y) * z} :: (x - y) * z == x * z - y * z
   {
-    lemma_mul_successor();
+    lemmaMulSuccessor();
     forall x:int, y:int, z:int
       ensures (x + y) * z == x * z + y * z
       ensures (x - y) * z == x * z - y * z
@@ -88,58 +88,58 @@ module MulInternals {
       assert forall i {:trigger (x + (i - 1)) * z} :: (x + (i - 1)) * z == ((x + i) - 1) * z == (x + i) * z - z;
       assert forall i {:trigger (x - (i + 1)) * z} :: (x - (i + 1)) * z == ((x - i) - 1) * z == (x - i) * z - z;
       assert forall i {:trigger (x - (i - 1)) * z} :: (x - (i - 1)) * z == ((x - i) + 1) * z == (x - i) * z + z;
-      lemma_mul_induction(f1);
-      lemma_mul_induction(f2);
+      lemmaMulInduction(f1);
+      lemmaMulInduction(f2);
       assert f1(y);
       assert f2(y);
     }
   }
 
   /* groups distributive and associative properties of multiplication */
-  predicate mul_auto()
+  predicate mulAuto()
   {
     && (forall x:int, y:int {:trigger x * y} :: x * y == y * x)
     && (forall x:int, y:int, z:int {:trigger (x + y) * z} :: (x + y) * z == x * z + y * z)
     && (forall x:int, y:int, z:int {:trigger (x - y) * z} :: (x - y) * z == x * z - y * z)
   }
 
-  /* proves that mul_auto is valid */
-  lemma lemma_mul_auto()
-    ensures  mul_auto()
+  /* proves that mulAuto is valid */
+  lemma lemmaMulAuto()
+    ensures  mulAuto()
   {
-    lemma_mul_commutes();
-    lemma_mul_distributes();
+    lemmaMulCommutes();
+    lemmaMulDistributes();
   }
 
   /* performs auto induction for multiplication */
-  lemma lemma_mul_induction_auto(x: int, f: int -> bool)
-    requires mul_auto() ==> f(0)
-                          && (forall i {:trigger is_le(0, i)} :: is_le(0, i) && f(i) ==> f(i + 1))
-                          && (forall i {:trigger is_le(i, 0)} :: is_le(i, 0) && f(i) ==> f(i - 1))
-    ensures  mul_auto()
+  lemma lemmaMulInductionAuto(x: int, f: int -> bool)
+    requires mulAuto() ==> f(0)
+                          && (forall i {:trigger isLe(0, i)} :: isLe(0, i) && f(i) ==> f(i + 1))
+                          && (forall i {:trigger isLe(i, 0)} :: isLe(i, 0) && f(i) ==> f(i - 1))
+    ensures  mulAuto()
     ensures  f(x)
   {
-    lemma_mul_commutes();
-    lemma_mul_distributes();
-    assert forall i {:trigger f(i)} :: is_le(0, i) && f(i) ==> f(i + 1);
-    assert forall i {:trigger f(i)} :: is_le(i, 0) && f(i) ==> f(i - 1);
-    lemma_mul_induction(f);
+    lemmaMulCommutes();
+    lemmaMulDistributes();
+    assert forall i {:trigger f(i)} :: isLe(0, i) && f(i) ==> f(i + 1);
+    assert forall i {:trigger f(i)} :: isLe(i, 0) && f(i) ==> f(i - 1);
+    lemmaMulInduction(f);
     assert f(x);
   }
 
   /* performs auto induction on multiplication for all i s.t. f(i) exists */
-  lemma lemma_mul_induction_auto_forall(f: int -> bool)
-    requires mul_auto() ==> f(0)
-                          && (forall i {:trigger is_le(0, i)} :: is_le(0, i) && f(i) ==> f(i + 1))
-                          && (forall i {:trigger is_le(i, 0)} :: is_le(i, 0) && f(i) ==> f(i - 1))
-    ensures  mul_auto()
+  lemma lemmaMulInductionAutoForall(f: int -> bool)
+    requires mulAuto() ==> f(0)
+                          && (forall i {:trigger isLe(0, i)} :: isLe(0, i) && f(i) ==> f(i + 1))
+                          && (forall i {:trigger isLe(i, 0)} :: isLe(i, 0) && f(i) ==> f(i - 1))
+    ensures  mulAuto()
     ensures  forall i {:trigger f(i)} :: f(i)
   {
-    lemma_mul_commutes();
-    lemma_mul_distributes();
-    assert forall i {:trigger f(i)} :: is_le(0, i) && f(i) ==> f(i + 1);
-    assert forall i {:trigger f(i)} :: is_le(i, 0) && f(i) ==> f(i - 1);
-    lemma_mul_induction(f);
+    lemmaMulCommutes();
+    lemmaMulDistributes();
+    assert forall i {:trigger f(i)} :: isLe(0, i) && f(i) ==> f(i + 1);
+    assert forall i {:trigger f(i)} :: isLe(i, 0) && f(i) ==> f(i - 1);
+    lemmaMulInduction(f);
   } 
 
 } 
