src/NonlinearArithmetic/Internals/ModInternalsNonlinear.dfy
@@ -17,27 +17,27 @@ module ModInternalsNonlinear {
   is highly unstable! */
 
   /* the remainder of 0 divided by an integer is 0 */
-  lemma lemma_mod_of_zero_is_zero(m:int)
+  lemma lemmaModOfZeroIsZero(m:int)
     requires 0 < m
     ensures 0 % m == 0
   { 
   }
 
   /* describes fundementals of the modulus operator */
-  lemma lemma_fundamental_div_mod(x:int, d:int)
+  lemma lemmaFundamentalDivMod(x:int, d:int)
     requires d != 0
     ensures x == d * (x / d) + (x % d)
   {
   }
 
   /* the remained of 0 divided by any integer is always 0 */
-  lemma lemma_0_mod_anything()
+  lemma lemma0ModAnything()
     ensures forall m: int {:trigger 0 % m} :: m > 0 ==> 0 % m == 0
   {
   }
 
   /* a natural number x divided by a larger natural number gives a remainder equal to x */
-  lemma lemma_small_mod(x:nat, m:nat)
+  lemma lemmaSmallMod(x:nat, m:nat)
     requires x < m
     requires 0 < m
     ensures x % m == x
@@ -45,7 +45,7 @@ module ModInternalsNonlinear {
   }
 
   /* the range of the modulus of any integer will be [0, m) where m is the divisor */
-  lemma lemma_mod_range(x:int, m:int)
+  lemma lemmaModRange(x:int, m:int)
     requires m > 0
     ensures 0 <= x % m < m
   {
