src/NonlinearArithmetic/Internals/MulInternalsNonlinear.dfy
@@ -17,27 +17,27 @@ module MulInternalsNonlinear {
   is highly unstable! */
 
   /* multiplying two positive integers will result in a positive integer */
-  lemma lemma_mul_strictly_positive(x: int, y: int)
+  lemma lemmaMulStrictlyPositive(x: int, y: int)
     ensures (0 < x && 0 < y) ==> (0 < x * y)
   {}
 
   /* multiplying two nonzero integers will never result in 0 as the poduct */
-  lemma lemma_mul_nonzero(x: int, y: int)
+  lemma lemmaMulNonzero(x: int, y: int)
     ensures x * y != 0 <==> x != 0 && y != 0
   {}
 
   /* multiplication is associative */
-  lemma lemma_mul_is_associative(x: int, y: int, z: int)
+  lemma lemmaMulIsAssociative(x: int, y: int, z: int)
     ensures x * (y * z) == (x * y) * z
   {}
 
   /* multiplication is distributive */
-  lemma lemma_mul_is_distributive_add(x: int, y: int, z: int)
+  lemma lemmaMulIsDistributiveAdd(x: int, y: int, z: int)
     ensures x * (y + z) == x * y + x * z
   {}
 
   /* the product of two integers is greater than the value of each individual integer */ 
-  lemma lemma_mul_ordering(x: int, y: int)
+  lemma lemmaMulOrdering(x: int, y: int)
     requires x != 0
     requires y != 0
     requires 0 <= x * y
@@ -45,7 +45,7 @@ module MulInternalsNonlinear {
   {}
 
   /* multiplying by a positive integer preserves inequality */
-  lemma lemma_mul_strict_inequality(x: int, y: int, z: int)
+  lemma lemmaMulStrictInequality(x: int, y: int, z: int)
     requires x < y
     requires z > 0
     ensures  x * z < y * z
