src/NonlinearArithmetic/Power.dfy
@@ -9,7 +9,7 @@
 *  SPDX-License-Identifier: MIT 
 ************************************************************************************/
 
-/* Every lemma comes in 2 forms: 'lemma_property' and 'lemma_property_auto'. The former takes arguments and may 
+/* Every lemma comes in 2 forms: 'lemmaProperty' and 'lemmaPropertyAuto'. The former takes arguments and may 
 be more stable and less reliant on Z3 heuristics. The latter includes automation and its use requires less effort */
 
 include "DivMod.dfy"
@@ -35,295 +35,295 @@ module Power {
   }
 
   /* A number raised to the power of 0 equals 1. */
-  lemma lemma_power_0(b: int)
+  lemma lemmaPower0(b: int)
     ensures power(b, 0) == 1
   {
-    reveal_power();
+    reveal power();
   }
 
-  lemma lemma_power_0_auto()
+  lemma lemmaPower0Auto()
     ensures forall b: nat {:trigger power(b, 0)} :: power(b, 0) == 1
   {
-    reveal_power();
+    reveal power();
     forall b: nat {:trigger power(b, 0)}
       ensures power(b, 0) == 1
     {
-      lemma_power_0(b);
+      lemmaPower0(b);
     }
   }
 
   /* A number raised to the power of 1 equals the number itself. */
-  lemma lemma_power_1(b: int)
+  lemma lemmaPower1(b: int)
     ensures power(b, 1) == b
   {
     calc {
       power(b, 1);
-        { reveal_power(); }
+        { reveal power(); }
       b * power(b, 0);
-        { lemma_power_0(b); }
+        { lemmaPower0(b); }
       b * 1;
-        { lemma_mul_basics_auto(); }
+        { lemmaMulBasicsAuto(); }
       b;
     }
   }
 
-  lemma lemma_power_1_auto()
+  lemma lemmaPower1Auto()
     ensures forall b: nat {:trigger power(b, 1)} :: power(b, 1) == b
   {
-    reveal_power();
+    reveal power();
     forall b: nat {:trigger power(b, 1)}
       ensures power(b, 1) == b
     {
-      lemma_power_1(b);
+      lemmaPower1(b);
     }
   }
 
   /* 0 raised to a positive power equals 0. */
-  lemma lemma_0_power(e: nat)
+  lemma lemma0Power(e: nat)
     requires e > 0
     ensures power(0, e) == 0
   {
-    reveal_power();
-    lemma_mul_basics_auto();
+    reveal power();
+    lemmaMulBasicsAuto();
     if e != 1 {
-      lemma_0_power(e - 1);
+      lemma0Power(e - 1);
     }
   }
 
-  lemma lemma_0_power_auto()
+  lemma lemma0PowerAuto()
     ensures forall e: nat {:trigger power(0, e)} :: e > 0 ==> power(0, e) == 0
   {
-    reveal_power();
+    reveal power();
     forall e: nat {:trigger power(0, e)} | e > 0
       ensures power(0, e) == 0
     {
-      lemma_0_power(e);
+      lemma0Power(e);
     }
   }
 
   /* 1 raised to any power equals 1. */
-  lemma lemma_1_power(e: nat)
+  lemma lemma1Power(e: nat)
     ensures power(1, e) == 1
   {
-    reveal_power();
-    lemma_mul_basics_auto();
+    reveal power();
+    lemmaMulBasicsAuto();
     if e != 0 {
-      lemma_1_power(e - 1);
+      lemma1Power(e - 1);
     }
   }
 
-  lemma lemma_1_power_auto()
+  lemma lemma1PowerAuto()
     ensures forall e: nat {:trigger power(1, e)} :: power(1, e) == 1
   {
-    reveal_power();
+    reveal power();
     forall e: nat {:trigger power(1, e)}
       ensures power(1, e) == 1
     {
-      lemma_1_power(e);
+      lemma1Power(e);
     }
   }
 
   /* Squaring a number is equal to raising it to the power of 2. */
-  lemma lemma_square_is_power_2(x: nat)
+  lemma lemmaSquareIsPower2(x: nat)
     ensures power(x, 2) == x * x
   {
-    reveal_power();
+    reveal power();
   }
 
-  lemma lemma_square_is_power_2_auto()
+  lemma lemmaSquareIsPower2Auto()
     ensures forall x: nat {:trigger power(x, 2)} :: power(x, 2) == x * x
   {
-    reveal_power();
+    reveal power();
     forall x: nat {:trigger power(x, 2)}
       ensures power(x, 2) == x * x
     {}
   }
 
   /* A positive number raised to any power is positive. */
-  lemma lemma_power_positive(b: int, e: nat)
+  lemma lemmaPowerPositive(b: int, e: nat)
     requires b > 0
     ensures 0 < power(b, e)
   {
-    lemma_mul_increases_auto();
-    lemma_mul_induction_auto(e, u => 0 <= u ==> 0 < power(b, u));
+    lemmaMulIncreasesAuto();
+    lemmaMulInductionAuto(e, u => 0 <= u ==> 0 < power(b, u));
   }
 
-  lemma lemma_power_positive_auto()
+  lemma lemmaPowerPositiveAuto()
     ensures forall b: int, e: nat {:trigger power(b, e)}
       :: b > 0 ==> 0 < power(b, e)
   {
-    reveal_power();
+    reveal power();
     forall b: int, e: nat {:trigger power(b, e)} | b > 0
       ensures 0 < power(b, e)
     {
-      lemma_power_positive(b, e);
+      lemmaPowerPositive(b, e);
     }
   }
 
   /* Add exponents when multiplying powers with the same base. */
-  lemma lemma_power_adds(b: int, e1: nat, e2: nat)
+  lemma lemmaPowerAdds(b: int, e1: nat, e2: nat)
     decreases e1
     ensures power(b, e1 + e2) == power(b, e1) * power(b, e2)
   {
     if e1 == 0 {
       calc {
         power(b, e1) * power(b, e2);
-          { lemma_power_0(b); }
+          { lemmaPower0(b); }
         1 * power(b, e2);
-          { lemma_mul_basics_auto(); }
+          { lemmaMulBasicsAuto(); }
         power(b, 0 + e2);
       }
     }
     else {
       calc {
         power(b, e1) * power(b, e2);
-          { reveal_power(); }
+          { reveal power(); }
         (b * power(b, e1 - 1)) * power(b, e2);
-          { lemma_mul_is_associative_auto(); }
+          { lemmaMulIsAssociativeAuto(); }
         b * (power(b, e1 - 1) * power(b, e2));
-          { lemma_power_adds(b, e1 - 1, e2); }
+          { lemmaPowerAdds(b, e1 - 1, e2); }
         b * power(b, e1 - 1 + e2);
-          { reveal_power(); }
+          { reveal power(); }
         power(b, e1 + e2);
       }
     }
   }
 
-  lemma lemma_power_adds_auto()
+  lemma lemmaPowerAddsAuto()
     ensures forall b: int, e1: nat, e2: nat {:trigger power(b, e1 + e2)}
       :: power(b, e1 + e2) == power(b, e1) * power(b, e2)
   {
-    reveal_power();
+    reveal power();
     forall b: int, e1: nat, e2: nat {:trigger power(b, e1 + e2)}
       ensures power(b, e1 + e2) == power(b, e1) * power(b, e2)
     {
-      lemma_power_adds(b, e1, e2);
+      lemmaPowerAdds(b, e1, e2);
     }
   }
 
   /* Subtract exponents when dividing powers. */
-  lemma lemma_power_subtracts(b: nat, e1: nat, e2: nat)
+  lemma lemmaPowerSubtracts(b: nat, e1: nat, e2: nat)
     requires b > 0
     requires e1 <= e2
     ensures power(b, e1) > 0
     ensures power(b, e2 - e1) == power(b, e2) / power(b, e1) > 0
   {
-    lemma_power_positive_auto();
+    lemmaPowerPositiveAuto();
     calc {
       power(b, e2) / power(b, e1);
-        { lemma_power_adds(b, e2 - e1, e1); }
+        { lemmaPowerAdds(b, e2 - e1, e1); }
       power(b, e2 - e1) * power(b, e1) / power(b, e1);
-        { lemma_div_by_multiple(power(b, e2 - e1), power(b, e1)); }
+        { lemmaDivByMultiple(power(b, e2 - e1), power(b, e1)); }
       power(b, e2 - e1);
     }
   }
 
-  lemma lemma_power_subtracts_auto()
+  lemma lemmaPowerSubtractsAuto()
     ensures forall b: nat, e1: nat :: b > 0 ==> power(b, e1) > 0
     ensures forall b: nat, e1: nat, e2: nat {:trigger power(b, e2 - e1)}
       :: b > 0 && e1 <= e2 ==>
          power(b, e2 - e1) == power(b, e2) / power(b, e1) > 0
   {
-    reveal_power();
-    lemma_power_positive_auto();
+    reveal power();
+    lemmaPowerPositiveAuto();
     forall b: nat, e1: nat, e2: nat {:trigger power(b, e2 - e1)}
       | b > 0 && e1 <= e2
       ensures power(b, e2 - e1) == power(b, e2) / power(b, e1) > 0
     {
-      lemma_power_subtracts(b, e1, e2);
+      lemmaPowerSubtracts(b, e1, e2);
     }
   }
 
   /* Multiply exponents when finding the power of a power. */
-  lemma lemma_power_multiplies(a: int, b: nat, c: nat)
+  lemma lemmaPowerMultiplies(a: int, b: nat, c: nat)
     decreases c
     ensures 0 <= b * c
     ensures power(power(a, b), c) == power(a, b * c)
   {
-    lemma_mul_nonnegative(b, c);
+    lemmaMulNonnegative(b, c);
     if c == 0 {
-      lemma_mul_basics_auto();
+      lemmaMulBasicsAuto();
       calc {
         power(a, b * c);
-          { lemma_power_0(a); }
+          { lemmaPower0(a); }
         1;
-          { lemma_power_0(power(a, b)); }
+          { lemmaPower0(power(a, b)); }
         power(power(a, b), c);
       }
     }
     else {
       calc {
         b * c - b;
-          { lemma_mul_basics_auto(); }
+          { lemmaMulBasicsAuto(); }
         b * c - b * 1;
-          { lemma_mul_is_distributive_auto(); }
+          { lemmaMulIsDistributiveAuto(); }
         b * (c - 1);
       }
-      lemma_mul_nonnegative(b, c - 1);
+      lemmaMulNonnegative(b, c - 1);
       assert 0 <= b * c - b;
 
       calc {
         power(a, b * c);
         power(a, b + b * c - b);
-          { lemma_power_adds(a, b, b * c - b); }
+          { lemmaPowerAdds(a, b, b * c - b); }
         power(a, b) * power(a, b * c - b);
         power(a, b) * power(a, b * (c - 1));
-          { lemma_power_multiplies(a, b, c - 1); }
+          { lemmaPowerMultiplies(a, b, c - 1); }
         power(a, b) * power(power(a, b), c - 1);
-          { reveal_power(); }
+          { reveal power(); }
         power(power(a, b), c);
       }
     }
   }
 
-  lemma lemma_power_multiplies_auto()
+  lemma lemmaPowerMultipliesAuto()
     ensures forall b: nat, c: nat {:trigger b * c} :: 0 <= b * c
     ensures forall a: int, b: nat, c: nat {:trigger power(a, b * c)}
       :: power(power(a, b), c) == power(a, b * c)
   {
-    reveal_power();
-    lemma_mul_nonnegative_auto();
+    reveal power();
+    lemmaMulNonnegativeAuto();
     forall a: int, b: nat, c: nat {:trigger power(a, b * c)}
       ensures power(power(a, b), c) == power(a, b * c)
     {
-      lemma_power_multiplies(a, b, c);
+      lemmaPowerMultiplies(a, b, c);
     }
   }
 
   /* Distribute the power to factors of a product. */
-  lemma lemma_power_distributes(a: int, b: int, e: nat)
+  lemma lemmaPowerDistributes(a: int, b: int, e: nat)
     decreases e
     ensures power(a * b, e) == power(a, e) * power(b, e)
   {
-    reveal_power();
-    lemma_mul_basics_auto();
+    reveal power();
+    lemmaMulBasicsAuto();
     if e > 0 {
       calc {
         power(a * b, e);
         (a * b) * power(a * b, e - 1);
-          { lemma_power_distributes(a, b, e - 1); }
+          { lemmaPowerDistributes(a, b, e - 1); }
         (a * b) * (power(a, e - 1) * power(b, e - 1));
-          { lemma_mul_is_associative_auto(); lemma_mul_is_commutative_auto(); }
+          { lemmaMulIsAssociativeAuto(); lemmaMulIsCommutativeAuto(); }
         (a * power(a, e - 1)) * (b * power(b, e - 1));
         power(a, e) * power(b, e);
       }
     }
   }
 
-  lemma lemma_power_distributes_auto()
+  lemma lemmaPowerDistributesAuto()
     ensures forall a: int, b: int, e: nat {:trigger power(a * b, e)}
       :: power(a * b, e) == power(a, e) * power(b, e)
   {
-    reveal_power();
+    reveal power();
     forall a: int, b: int, e: nat {:trigger power(a * b, e)}
       ensures power(a * b, e) == power(a, e) * power(b, e)
     {
-      lemma_power_distributes(a, b, e);
+      lemmaPowerDistributes(a, b, e);
     }
   }
 
   /* Group properties of powers. */
-  lemma lemma_power_auto()
+  lemma lemmaPowerAuto()
     ensures forall x: int {:trigger power(x, 0)} :: power(x, 0) == 1
     ensures forall x: int {:trigger power(x, 1)} :: power(x, 1) == x
     ensures forall x: int, y: int {:trigger power(x, y)} :: y == 0 ==> power(x, y) == 1
@@ -334,233 +334,233 @@ module Power {
     ensures forall x: int, y: nat, z: nat {:trigger power(x, y - z)} :: y >= z ==> power(x, y - z) * power(x, z) == power(x, y)
     ensures forall x: int, y: int, z: nat {:trigger power(x * y, z)} :: power(x * y, z) == power(x, z) * power(y, z)
   {
-    reveal_power();
+    reveal power();
 
-    lemma_power_0_auto();
-    lemma_power_1_auto();
+    lemmaPower0Auto();
+    lemmaPower1Auto();
 
-    lemma_power_distributes_auto();
-    lemma_power_adds_auto();
+    lemmaPowerDistributesAuto();
+    lemmaPowerAddsAuto();
 
     forall x: int, y: nat, z: nat {:trigger power(x, y - z)} | y >= z
       ensures power(x, y - z) * power(x, z) == power(x, y)
     {
-      lemma_power_adds(x, y - z, z);
+      lemmaPowerAdds(x, y - z, z);
     }
 
-    lemma_mul_auto();
-    lemma_mul_increases_auto();
-    lemma_mul_strictly_increases_auto();
+    lemmaMulAuto();
+    lemmaMulIncreasesAuto();
+    lemmaMulStrictlyIncreasesAuto();
   }
 
   /* A positive number raised to a power strictly increases as the power
   strictly increases. */
-  lemma lemma_power_strictly_increases(b: nat, e1: nat, e2: nat)
+  lemma lemmaPowerStrictlyIncreases(b: nat, e1: nat, e2: nat)
     requires 1 < b
     requires e1 < e2
     ensures power(b, e1) < power(b, e2)
   {
-    lemma_power_auto();
+    lemmaPowerAuto();
     var f := e => 0 < e ==> power(b, e1) < power(b, e1 + e);
-    forall i {:trigger is_le(0, i)} | is_le(0, i) && f(i)
+    forall i {:trigger isLe(0, i)} | isLe(0, i) && f(i)
       ensures f(i + 1)
     {
       calc {
         power(b, e1 + i);
-        <= { lemma_power_positive(b, e1 + i);
-             lemma_mul_left_inequality(power(b, e1 + i), 1, b); }
+        <= { lemmaPowerPositive(b, e1 + i);
+             lemmaMulLeftInequality(power(b, e1 + i), 1, b); }
           power(b, e1 + i) * b;
-        == { lemma_power_1(b); }
+        == { lemmaPower1(b); }
           power(b, e1 + i) * power(b, 1);
-        == { lemma_power_adds(b, e1 + i, 1); }
+        == { lemmaPowerAdds(b, e1 + i, 1); }
           power(b, e1 + i + 1);
       }
     }
-    lemma_mul_induction_auto(e2 - e1, f);
+    lemmaMulInductionAuto(e2 - e1, f);
   }
 
-  lemma lemma_power_strictly_increases_auto()
+  lemma lemmaPowerStrictlyIncreasesAuto()
     ensures forall b: nat, e1: nat, e2: nat {:trigger power(b, e1),
       power(b, e2)} :: (1 < b && e1 < e2) ==> power(b, e1) < power(b, e2)
   {
-    reveal_power();
+    reveal power();
     forall b: nat, e1: nat, e2: nat {:trigger power(b, e1), power(b, e2)}
       | 1 < b && e1 < e2
       ensures power(b, e1) < power(b, e2)
     {
-      lemma_power_strictly_increases(b, e1, e2);
+      lemmaPowerStrictlyIncreases(b, e1, e2);
     }
   }
 
   /* A positive number raised to a power increases as the power increases. */
-  lemma lemma_power_increases(b: nat, e1: nat, e2: nat)
+  lemma lemmaPowerIncreases(b: nat, e1: nat, e2: nat)
     requires b > 0
     requires e1 <= e2
     ensures power(b, e1) <= power(b, e2)
   {
-    lemma_power_auto();
+    lemmaPowerAuto();
     var f := e => 0 <= e ==> power(b, e1) <= power(b, e1 + e);
-    forall i {:trigger is_le(0, i)} | is_le(0, i) && f(i)
+    forall i {:trigger isLe(0, i)} | isLe(0, i) && f(i)
       ensures f(i + 1)
     {
       calc {
         power(b, e1 + i);
-        <= { lemma_power_positive(b, e1 + i);
-             lemma_mul_left_inequality(power(b, e1 + i), 1, b); }
+        <= { lemmaPowerPositive(b, e1 + i);
+             lemmaMulLeftInequality(power(b, e1 + i), 1, b); }
           power(b, e1 + i) * b;
-        == { lemma_power_1(b); }
+        == { lemmaPower1(b); }
           power(b, e1 + i) * power(b, 1);
-        == { lemma_power_adds(b, e1 + i, 1); }
+        == { lemmaPowerAdds(b, e1 + i, 1); }
           power(b, e1 + i + 1);
       }
     }
-    lemma_mul_induction_auto(e2 - e1, f);
+    lemmaMulInductionAuto(e2 - e1, f);
   }
 
-  lemma lemma_power_increases_auto()
+  lemma lemmaPowerIncreasesAuto()
     ensures forall b: nat, e1: nat, e2: nat {:trigger power(b, e1),
       power(b, e2)} :: (1 < b && e1 <= e2) ==> power(b, e1) <= power(b, e2)
   {
-    reveal_power();
+    reveal power();
     forall b: nat, e1: nat, e2: nat {:trigger power(b, e1), power(b, e2)}
       | 1 < b && e1 <= e2
       ensures power(b, e1) <= power(b, e2)
     {
-      lemma_power_increases(b, e1, e2);
+      lemmaPowerIncreases(b, e1, e2);
     }
   }
 
   /* A power strictly increases as a positive number raised to the power
   strictly increases. */
-  lemma lemma_power_strictly_increases_converse(b: nat, e1: nat, e2: nat)
+  lemma lemmaPowerStrictlyIncreasesConverse(b: nat, e1: nat, e2: nat)
     requires b > 0
     requires power(b, e1) < power(b, e2)
     ensures e1 < e2
   {
     if e1 >= e2 {
-      lemma_power_increases(b, e2, e1);
+      lemmaPowerIncreases(b, e2, e1);
       assert false;
     }
   }
 
-  lemma lemma_power_strictly_increases_converse_auto()
+  lemma lemmaPowerStrictlyIncreasesConverseAuto()
     ensures forall b: nat, e1: nat, e2: nat
       {:trigger power(b, e1), power(b, e2)}
       :: b > 0 && power(b, e1) < power(b, e2) ==> e1 < e2
   {
-    reveal_power();
+    reveal power();
     forall b: nat, e1: nat, e2: nat {:trigger power(b, e1), power(b, e2)}
       | b > 0 && power(b, e1) < power(b, e2)
       ensures e1 < e2
     {
-      lemma_power_strictly_increases_converse(b, e1, e2);
+      lemmaPowerStrictlyIncreasesConverse(b, e1, e2);
     }
   }
 
   /* A power increases as a positive number raised to the power increases. */
-  lemma lemma_power_increases_converse(b: nat, e1: nat, e2: nat)
+  lemma lemmaPowerIncreasesConverse(b: nat, e1: nat, e2: nat)
     requires 1 < b
     requires power(b, e1) <= power(b, e2)
     ensures e1 <= e2
   {
     if e1 > e2 {
-      lemma_power_strictly_increases(b, e2, e1);
+      lemmaPowerStrictlyIncreases(b, e2, e1);
       assert false;
     }
   }
 
-  lemma lemma_power_increases_converse_auto()
+  lemma lemmaPowerIncreasesConverseAuto()
     ensures forall b: nat, e1: nat, e2: nat
       {:trigger power(b, e1), power(b, e2)}
       :: 1 < b && power(b, e1) <= power(b, e2) ==> e1 <= e2
   {
-    reveal_power();
+    reveal power();
     forall b: nat, e1: nat, e2: nat {:trigger power(b, e1), power(b, e2)}
       | 1 < b && power(b, e1) <= power(b, e2)
       ensures e1 <= e2
     {
-      lemma_power_increases_converse(b, e1, e2);
+      lemmaPowerIncreasesConverse(b, e1, e2);
     }
   }
 
   /* (b^xy)^z = (b^x)^yz */
-  lemma lemma_pull_out_powers(b: nat, x: nat, y: nat, z: nat)
+  lemma lemmaPullOutPowers(b: nat, x: nat, y: nat, z: nat)
     requires b > 0
     ensures 0 <= x * y
     ensures 0 <= y * z
     ensures power(power(b, x * y), z) == power(power(b, x), y * z)
   {
-    lemma_mul_nonnegative(x, y);
-    lemma_mul_nonnegative(y, z);
-    lemma_power_positive(b, x);
+    lemmaMulNonnegative(x, y);
+    lemmaMulNonnegative(y, z);
+    lemmaPowerPositive(b, x);
     calc {
       power(power(b, x * y), z);
-        { lemma_power_multiplies(b, x, y); }
+        { lemmaPowerMultiplies(b, x, y); }
       power(power(power(b, x), y), z);
-        { lemma_power_multiplies(power(b, x), y, z); }
+        { lemmaPowerMultiplies(power(b, x), y, z); }
       power(power(b, x), y * z);
     }
   }
 
-  lemma lemma_pull_out_powers_auto()
+  lemma lemmaPullOutPowersAuto()
     ensures forall y: nat, z: nat {:trigger z * y} :: 0 <= z * y && 0 <= y * z
     ensures forall b: nat, x: nat, y: nat, z: nat
       {:trigger power(power(b, x * y), z)}
       :: b > 0 ==> power(power(b, x * y), z) == power(power(b, x), y * z)
   {
-    reveal_power();
-    lemma_mul_nonnegative_auto();
+    reveal power();
+    lemmaMulNonnegativeAuto();
     forall b: nat, x: nat, y: nat, z: nat {:trigger power(power(b, x * y), z)}
       | b > 0 ensures power(power(b, x * y), z) == power(power(b, x), y * z)
     {
-      lemma_pull_out_powers(b, x, y, z);
+      lemmaPullOutPowers(b, x, y, z);
     }
   }
 
   /* Inequality due to smaller numerator, same denominator. */
-  lemma lemma_power_division_inequality(x: nat, b: nat, e1: nat, e2: nat)
+  lemma lemmaPowerDivisionInequality(x: nat, b: nat, e1: nat, e2: nat)
     requires b > 0
     requires e2 <= e1
     requires x < power(b, e1)
     ensures power(b, e2) > 0
     ensures x / power(b, e2) < power(b, e1 - e2)
   {
-    lemma_power_positive_auto();
+    lemmaPowerPositiveAuto();
     calc ==> {
       x / power(b, e2) >= power(b, e1 - e2);
-        { lemma_mul_inequality(power(b, e1 - e2), x / power(b, e2), power(b, e2)); }
+        { lemmaMulInequality(power(b, e1 - e2), x / power(b, e2), power(b, e2)); }
       x / power(b, e2) * power(b, e2) >= power(b, e1 - e2) * power(b, e2);
-        { lemma_fundamental_div_mod(x, power(b, e2));
-          lemma_mul_is_commutative_auto(); }
+        { lemmaFundamentalDivMod(x, power(b, e2));
+          lemmaMulIsCommutativeAuto(); }
       x - x % power(b, e2) >= power(b, e1 - e2) * power(b, e2);
-        { lemma_power_adds(b, e1 - e2, e2); }
+        { lemmaPowerAdds(b, e1 - e2, e2); }
       x - x % power(b, e2) >= power(b, e1);
-        { lemma_mod_properties_auto(); }
+        { lemmaModPropertiesAuto(); }
       x >= power(b, e1);
       false;
     }
   }
 
-  lemma lemma_power_division_inequality_auto()
+  lemma lemmaPowerDivisionInequalityAuto()
     ensures forall b: nat, e2: nat :: b > 0 ==> power(b, e2) > 0
     ensures forall x: nat, b: nat, e1: nat, e2: nat
       {:trigger x / power(b, e2), power(b, e1 - e2)}
       :: b > 0 && e2 <= e1 && x < power(b, e1) ==>
          x / power(b, e2) < power(b, e1 - e2)
   {
-    reveal_power();
-    lemma_power_positive_auto();
+    reveal power();
+    lemmaPowerPositiveAuto();
     forall x: nat, b: nat, e1: nat, e2: nat
       {:trigger x / power(b, e2), power(b, e1 - e2)}
       | b > 0 && e2 <= e1 && x < power(b, e1)
       ensures x / power(b, e2) < power(b, e1 - e2)
     {
-      lemma_power_division_inequality(x, b, e1, e2);
+      lemmaPowerDivisionInequality(x, b, e1, e2);
     }
   }
 
   /* b^e % b = 0 */
-  lemma lemma_power_mod(b: nat, e: nat) 
+  lemma lemmaPowerMod(b: nat, e: nat) 
     requires b > 0 && e > 0
     ensures power(b, e) % b == 0;
   {
@@ -568,45 +568,45 @@ module Power {
     calc {
       power(b, e) % b;
       (b * power(b, e - 1)) % b;
-        { lemma_mul_is_associative_auto(); }
+        { lemmaMulIsAssociativeAuto(); }
       (power(b, e - 1) * b) % b;
         {
-          lemma_power_positive_auto();
-          lemma_mod_multiples_basic(power(b, e-1) , b);
+          lemmaPowerPositiveAuto();
+          lemmaModMultiplesBasic(power(b, e-1) , b);
         }
       0;
     }
   }
 
-  lemma lemma_power_mod_auto()
+  lemma lemmaPowerModAuto()
     ensures forall b: nat, e: nat {:trigger power(b, e)}
       :: b > 0 && e > 0 ==> power(b, e) % b == 0
   {
-    reveal_power();
+    reveal power();
     forall b: nat, e: nat {:trigger power(b, e)} | b > 0 && e > 0
       ensures power(b, e) % b == 0
     {
-      lemma_power_mod(b, e);
+      lemmaPowerMod(b, e);
     }
   }
 
   /* ((b % e)^e) % m = b^e % m */
-  lemma lemma_power_mod_noop(b: int, e: nat, m: int)
+  lemma lemmaPowerModNoop(b: int, e: nat, m: int)
     decreases e
     requires m > 0
     ensures power(b % m, e) % m == power(b, e) % m
   {
     reveal power();
-    lemma_mod_properties_auto();
+    lemmaModPropertiesAuto();
     if e > 0 {
       calc {
         power(b % m, e) % m;
         ((b % m) * power(b % m, e - 1)) % m;
-          { lemma_mul_mod_noop_general(b, power(b % m, e - 1), m); }
+          { lemmaMulModNoopGeneral(b, power(b % m, e - 1), m); }
         ((b % m) * (power(b % m, e - 1) % m) % m) % m;
-          { lemma_power_mod_noop(b, e - 1, m); }
+          { lemmaPowerModNoop(b, e - 1, m); }
         ((b % m) * (power(b, e - 1) % m) % m) % m;
-          { lemma_mul_mod_noop_general(b, power(b, e - 1), m); }
+          { lemmaMulModNoopGeneral(b, power(b, e - 1), m); }
         (b * (power(b, e - 1)) % m) % m;
         (b * (power(b, e - 1))) % m;
         power(b, e) % m;
@@ -614,15 +614,15 @@ module Power {
     }
   }
 
-  lemma lemma_power_mod_noop_auto()
+  lemma lemmaPowerModNoopAuto()
     ensures forall b: nat, e: nat, m: nat {:trigger power(b % m, e)}
       :: m > 0 ==> power(b % m, e) % m == power(b, e) % m
   {
-    reveal_power();
+    reveal power();
     forall b: nat, e: nat, m: nat {:trigger power(b % m, e)}
       | m > 0 ensures power(b % m, e) % m == power(b, e) % m
     {
-      lemma_power_mod_noop(b, e, m);
+      lemmaPowerModNoop(b, e, m);
     }
   }
 
