src/OptionAndResult.dfy
@@ -8,30 +8,30 @@
 
 module OptionAndResult {
   
-  datatype Option<T, R> = None | Some(value: T) {
-    function method to_result(error: R): Result<T, R> 
+  datatype Option<T> = None | Some(value: T) {
+    function method toResult(): Result<T, string> 
     {
       match this
       case Some(v) => Success(v)
-      case None => Failure(error)
+      case None() => Failure("Option is None")
     }
     
-    function method unwrap_or(default: T): T 
+    function method unwrapOr(default: T): T 
     {
       match this
       case Some(v) => v
-      case None => default
+      case None() => default
     }
   }
   
   datatype Result<T, R> = | Success(value: T) | Failure(error: R) {
-    function method to_option(): Option<T, R> 
+    function method toOption(): Option<T> 
     {
       match this
       case Success(s) => Some(s)
       case Failure(e) => None()
     }
-    function method unwrap_or(default: T): T 
+    function method unwrapOr(default: T): T 
     {
       match this
       case Success(s) => s
